Start the injectivity proof, looks good

src/tls/HSL.Transcript.fst
@@ -59,6 +59,12 @@ val serialize_list_max_size
   ))
 //  [SMTPat (Seq.length (LP.serialize (LPSL.serialize_list _ s) x))]
 
+let serialize_client_hello (ch:CH.clientHello) =
+  LP.serialize HSM.handshake_serializer (HSM.M_client_hello ch)
+
+let serialize_server_hello (sh:SH.serverHello) =
+  LP.serialize HSM.handshake_serializer (HSM.M_server_hello sh)
+
 let serialize_retry (r:option retry)
   : GTot (b:bytes{Seq.length b < 2 * max_message_size })
   =
@@ -67,13 +73,7 @@ let serialize_retry (r:option retry)
   | Some (ht, sh) ->
     let ht = FStar.Bytes.hide ht in
     LP.serialize HSM.handshake_serializer (Parsers.Handshake.M_message_hash ht) `Seq.append`
-    LP.serialize SH.serverHello_serializer sh
-
-let serialize_client_hello (ch:CH.clientHello) =
-  LP.serialize HSM.handshake_serializer (HSM.M_client_hello ch)
-
-let serialize_server_hello (sh:SH.serverHello) =
-  LP.serialize HSM.handshake_serializer (HSM.M_server_hello sh)
+    serialize_server_hello sh
 
 let transcript_bytes (t:transcript_t)
   : GTot (b:bytes {
@@ -104,7 +104,56 @@ let transcript_bytes (t:transcript_t)
     serialize_server_hello sh `Seq.append`
     LP.serialize (LPSL.serialize_list _ HSM13.handshake13_serializer) rest
 
-let rec transcript_bytes_injective (t1 t2:transcript_t)
+let transcript_is_empty (t: transcript_t) : Tot bool = match t with
+  | Start None -> true
+  | _ -> false
+
+let transcript_get_retry (t: transcript_t) : Tot (option retry) = match t with
+  | Start r -> r
+  | TruncatedClientHello r _ -> r
+  | ClientHello r _ -> r
+  | Transcript12 _ _ _ -> None
+  | Transcript13 r _ _ _ -> r
+
+let transcript_set_retry (t: transcript_t) (r: option retry { Transcript12? t ==> None? r }) : Tot transcript_t =
+  match t with
+  | Start _ -> Start r
+  | TruncatedClientHello _ tch -> TruncatedClientHello r tch
+  | ClientHello _ ch -> ClientHello r ch
+  | Transcript12 ch sh rest -> Transcript12 ch sh rest
+  | Transcript13 _ ch sh rest -> Transcript13 r ch sh rest
+
+let transcript_script_bytes (t: transcript_t) : Lemma
+  (transcript_bytes t `Seq.equal` (serialize_retry (transcript_get_retry t) `Seq.append` transcript_bytes (transcript_set_retry t None)))
+= ()
+
+let transcript_bytes_does_not_start_with_message_hash
+  (t: transcript_t)
+  (r: retry)
+  (q: Seq.seq FStar.UInt8.t)
+: Lemma
+  (requires (transcript_get_retry t == None /\ transcript_bytes t == serialize_retry (Some r) `Seq.append` q))
+  (ensures False)
+= ()
+
+let transcript_bytes_injective_retry
+  (r1: option retry)
+  (t1: transcript_t { transcript_get_retry t1 == None } )
+  (r2: option retry)
+  (t2: transcript_t { transcript_get_retry t2 == None } )
+: Lemma
+  (requires (serialize_retry r1 `Seq.append` transcript_bytes t1 == serialize_retry r2 `Seq.append` transcript_bytes t2))
+  (ensures (r1 == r2 /\ transcript_bytes t1 `Seq.equal` transcript_bytes t2))
+= match r1, r2 with
+  | None, None ->
+    assert (transcript_bytes t1 `Seq.equal` (Seq.empty `Seq.append` transcript_bytes t1));
+    assert (transcript_bytes t2 `Seq.equal` (Seq.empty `Seq.append` transcript_bytes t2))
+  | Some (ht1, sh1), Some (ht2, sh2) ->
+    assert ((serialize_retry r1 `Seq.append` transcript_bytes t1) `Seq.equal` (LP.serialize HSM.handshake_serializer (HSM.M_message_hash (FStar.Bytes.hide ht1)) `Seq.append` (serialize_server_hello sh1 `Seq.append` transcript_bytes t1)));
+    assert ((serialize_retry r2 `Seq.append` transcript_bytes t2) `Seq.equal` (LP.serialize HSM.handshake_serializer (HSM.M_message_hash (FStar.Bytes.hide ht2)) `Seq.append` (serialize_server_hello sh2 `Seq.append` transcript_bytes t2)));
+    assume (r1 == r2 /\ transcript_bytes t1 == transcript_bytes t2)
+
+let transcript_bytes_injective (t1 t2:transcript_t)
   : Lemma
     (requires
       transcript_bytes t1 `Seq.equal` transcript_bytes t2)
